

Lang's Algebra Chapter 4 Solutions

Amanuel Tewodros

November 5, 2025

(1) We will show that $a \implies b \implies c \implies a$.

$a \implies b$ Suppose there is $g(X)$, $\deg g > 0$, such that $(g(X)) \supsetneq (f(X))$. This implies there is $h(X)$ such that $h(X)g(X) = f(X)$. By primality, $g(X) \notin (f(X))$, implies $h(X) \in (f(X))$. This implies $h(X)$ generates $(f(X))$ which implies $h(X) = cf(X)$ and $g(X) = d$ for some $d \in k$, a contradiction. Hence $(f(X))$ must be maximal.

$b \implies c$ If $f(X) = g(X)h(X)$, where neither $g(X)$ nor $h(X)$ are units, then $(g(X)) \supsetneq (f(X))$, contradicting the maximality of $(f(X))$.

$c \implies a$ Let $h(X) = r(X)s(X) \in (f(X))$. Since $k[X]$ is UFD and $f(X)|h(X)$, the prime factorization at least one of r and s contains $f(X)$ as a factor. WLOG, let $f(X) \mid r(X)$, then $r(X) \in (f(X))$ and thus $(f(X))$ is prime.

(2) (a) The equivalent statement for rational numbers is the following:

For a given rational number a/b and the set of primes P of \mathbb{Z} , we have

$$\frac{a}{b} = \sum_{p \in P} \frac{a_p}{p^{j_p}} + N,$$

where $j_p > 0$ if $a_p \neq 0$, $a_p = 0$ if $j_p = 0$, $a_p \leq p^{j_p}$ and N is an integer. This expression is unique.

First, we show that such expression exists. Let b be a product of two coprime numbers c and d . The by Euclid's algorithm, there are numbers x, y such that $cx + dy = a$. Substituting this in a/b , we see that

$$\frac{a}{b} = \frac{x}{d} + \frac{y}{c}.$$

And hence,

$$\frac{a}{b} = \sum_{p \in P} \frac{a_p}{p^{j_p}},$$

Where $a_p = 0$ if $j_p = 0$. If $a_p \geq p^{j_p}$, then we can write a_p/p^{j_p} as $a'_p/p^{j_p} + N_p$ for some $N_p > 0$ and $a_p < p^{j_p}$. Hence, the given expression exists. For uniqueness, let

$$\frac{a}{b} = \sum_{p \in P} \frac{a_p}{p^{j_p}} + N = \sum_{p \in P} \frac{b_p}{p^{i_p}} + M.$$

Fix a prime q and WLOG assume $j_q > i_q$. Then we have the following equation

$$\ell(a_q - p^{j_q-i_q}b_q) = q^{j_q}L,$$

where ℓ is the least common multiple of all $p^{j_p}, p \neq q$ and L is some integer. Since q^{j_q} divides the L.H.S but not ℓ and a_q , we have $j_q = i_q$. This implies

$$\frac{a_q - b_q}{q^{j_q}} = \sum_{p \neq q} \frac{b_p - a_p}{p^{j_p}} + M - N$$

Since $q \nmid p^{j_p}$ we have $b_p = a_p$ and since $|a_q - b_q| < p^{j_p}$, $M = N$. Hence, the expression is unique.

(b) The equivalent statement for positive integers is the following:

If $\alpha, \beta \in \mathbb{Z}$, such that $\beta > 1$, then there exist unique positive integers

$$\alpha_0, \alpha_1, \dots, \alpha_d \in \mathbb{Z},$$

such that $\alpha_i < \beta$ and

$$\alpha = \alpha_0 + \alpha_1\beta + \dots + \alpha_d\beta^d.$$

If $\alpha < \beta$, there is nothing to show. If $\beta \leq \alpha$, then by Euclid's algorithm, there are unique positive integers q and $r < \beta$ such that $\alpha = q\beta + r$ and $q < \alpha$. By induction, existence (and thus uniqueness) is proven.

(3) $f(X + Y) \bmod Y = f(X)$. Collecting similar powers of Y , we have the given expression. Now take the i -th derivative of $f(X + Y)$ with respect to Y

$$D^i f(X + Y) = \sum_{k=i}^n k! \phi_k(X) Y^{k-i}.$$

Substituting $Y = 0$, you get $D^i f(X) = i! \phi_i(X)$.

(4) First we introduce the notion of partial derivative similar to that in calculus as follows:

$$\frac{\partial}{\partial X_i} \left(\sum_{(v)} a_{(v)} X_1^{v_1} \dots X_n^{v_n} \right) = \begin{cases} \left(\sum_{(v)} a_{(v)} v_i X_1^{v_1} \dots X_i^{v_i-1} \dots X_n^{v_n} \right) & \text{if } v_i > 0, \\ 0 & \text{if otherwise.} \end{cases}$$

We define the Taylor expansion in n variables as a polynomial in $k[X_1, \dots, X_n, Y_1, \dots, Y_n]$ such that

$$f(X_1 + Y_1, \dots, X_n + Y_n) = f(X_1, \dots, X_n) + \sum_{(v)} \phi_{(v)}(X_1, \dots, X_n) Y_1^{v_1} \dots Y_n^{v_n}.$$

The above definition can be shown to be unambiguous using a similar proof as (3). Taking the v_i -th partial derivative of f with respect to X_i followed by substituting $Y_i = 0$ and rearranging terms the following relation is proved.

$$\phi_{(v)}(X_1, \dots, X_n) = \frac{1}{v_1! \dots v_n!} \frac{\partial^{v_1 + \dots + v_n} f}{\partial X_1^{v_1} \dots \partial X_n^{v_n}}$$

(5) (a) For $f(X) = X^4 + 1$, we notice that $f(X + 1) = X^4 + 4X^3 + 6X^2 + 4X + 2$ is irreducible over \mathbb{Z} by Eisenstein's criterion or irreducibility. For $g(X) = X^6 + X^3 + 1$, reducibility over \mathbb{Z} fails by the integral root test as $g(\pm 1) \neq 0$. Irreducibility over \mathbb{Q} directly follows from the irreducibility over \mathbb{Z} .

(b) If f is a reducible polynomial over k , say $f(X) = g(X)h(X)$, $\deg h, \deg g \geq 1$, then $\deg h + \deg g = 3$. This can only happen if either of h and g has degree 1. $X^3 - 5X^2 + 1$ fails irreducibility test by the integral root test thus not irreducible over \mathbb{Q} .

(c) Considering $X^2 + Y^2 - 1$ as an element of $K[Y][X]$, we see that $K[Y]$ is factorial and we can use Eisenstein's irreducibility test using the irreducible $Y - 1$ as p and we see that $Y - 1 \mid Y^2 - 1$, $(Y - 1)^2 \nmid Y^2 - 1$ and $Y - 1 \nmid 1$. Thus $X^2 + Y^2 - 1$ is irreducible over \mathbb{Q} and \mathbb{C} .

(6) Let $f(X) = a_0 + \dots + a_d X^d$. We can turn f to monic by factoring out a_d as $g(X) = f(X)/a_d = X^d + \frac{a_{d-1}}{a_d} X^{d-1} + \dots + \frac{a_0}{a_d}$. If t_1, \dots, t_m are the root of g , then we have $t_1 \dots t_m = a_0/a_d$. It then must be the case that for a root $t_i = x_i/y_i$, $x_i \mid a_0$ and $y_i \mid a_d$.

(7) (a) Suppose $(0, \dots, 0)$ is the only root of f . Since $a^{q-1} = 1$ for any finite field with q elements and $a \neq 0$,

$$1 - f(X)^{q-1} = \begin{cases} 1 & \text{if } X = 0, \\ 0 & \text{otherwise.} \end{cases}$$

Let $g(X_n) = 1 - f(X_1, \dots, X_n) \in k[X_1, \dots, X_{n-1}][X_n]$. This implies all the units u_1, \dots, u_{q-1} are zeros of g and $\prod_{k=1}^{q-1} (X_n - u_k)$ divides $g(X_n)$. This product is equal to $X_n^{q-1} - 1$. Doing this for all X_i , we see that

$$h(X) \prod_{s=1}^n 1 - X_s^{q-1} = (1 - f(X)^{q-1}).$$

The degree of the polynomial on the RHS $< n(q-1)$ where as that of the LHS is $\deg h + (q-1)n > (q-1)n$, a contradiction. Thus $f(X)$ must have a root other than 0.

- (b) If $q = 2$, the sum expression is obviously true. Otherwise note that u is unit iff $-u$ is unit in k and that $u^k = v^k$ iff $v = u$ if u and v are units. Thus the sum expression is true. By definition,

$$N = \sum_{x \in k^n} (1 - f(x)^{q-1}).$$

The second expression for $\prod_i \psi(i)$ directly follow from taking the sum fixing each x_k one by one and factoring out common units $x_1^{i_1} \cdots x_k^{i_k}$ for all valid k .

For the last part, we have

$$I = \{(i_1, \dots, i_n) \in \mathbb{Z}_{\geq 0}^n : i_1 + \dots + i_n \leq d(q-1)\}.$$

$$\begin{aligned} N &= \sum_{x \in k^n} (1 - f(x)^{q-1}) \\ &\equiv - \sum_{i \in I} c(i) \sum_{x \in k^n} x_1^{i_1} \cdots x_n^{i_n} \pmod{q} \\ &\equiv - \sum_{i \in I} c(i) \prod_{k=1}^n \psi(i_k) \pmod{q}. \end{aligned}$$

In the last term all exponents i_j can not be a multiple of $q-1$ because otherwise $\deg f \geq n$. Thus the product mod $q = 0$ and the statement is proved. dots

- (c) By assumption and (b) $f_1 \cdots f_r(a) = 0$ for some $a \neq 0$. This implies at least one $f_i(a) = 0$. But then $\sum_{k=1}^r \prod_{j \neq k} f_j(a) = \prod_{j=1, j \neq i}^r f_j(a)$ which implies we have $f_j \neq f_i$ such that $f_j(a) = 0$. Carrying out this process, we prove that a is shared across all a .
- (d) Let f be an arbitrary function from $k^n \rightarrow k$. Then we define the polynomial $g \in k[X_1, \dots, X_n]$ as

$$g(X_1, \dots, X_n) = \sum_{c \in k^n} f(c) (1 - \prod_{i=1}^n (X_i - c_i)^{q-1}).$$

It is clear $g = f$

- (8) The induced map is going to be the map $f(X) \mapsto f(aX + b)$ which also fixes the elements of A . The map is injective because if $f(aX + b) = 0$, then $f(X) = 0$ for infinitely many entries thus $f(X) = 0$. We also observe that $f(aX + b) = h(X)$, then $h(a^{-1}X - a^{-1}b) = f(X)$, making the induced map an automorphism with the inverse $f(X) \mapsto f(a^{-1}X - a^{-1}b)$.
- (9) Let f be an automorphism on $A[X]$. By bijectivity, for any $p \in A[X]$, we have $\deg f(p) = \deg p$. Thus $\deg f(X) = 1$ or $f(X) = aX + b$ for some $a, b \in A$. Now suppose $X = f(cX + d) = ac(X) + cb + d$. This implies $ac = 1$ and a must be a unit.
- (10) Let $X \mapsto p(X)/q(X) \in K(X)$ where p and q are coprime in $K[X]$. By surjectivity, we have $f(X) = \sum_{i=0}^{d'} a_i X^i, g(X) = \sum_{i=0}^d b_i X^i, a_{d'}, b_d \neq 0$ such that $f(\frac{p}{q}X)/g(\frac{p}{q}X) = X$. We note that

$$f(\frac{p}{q}X) = (\sum_{i=0}^{d'} a_i p^i(X) q^{d'-i}(X)) / q^{d'}(X)$$

. Similar thing can be said for $g(\frac{p}{q}X)$. By rearranging terms, we get the equation

$$x q^{d'}(X) \sum_{i=0}^d b_i p^i(X) q^{d-i}(X) = q^d(X) \sum_{i=0}^{d'} a_i p^i(X) q^{d'-i}(X). \quad (1)$$

We have three cases:

$d' < d$. Since $q^d(X)$ must divide the L.H.S, $q(X) \mid \sum_{i=0}^d b_i p^i(X) q^{d-i}(X)$ or $q(X) \mid x$. The former can only happen if $b_d = 0$ contradicting assumption. This implies $q(X) \mid x$ or in other words $q(X) = cX$ for some $c \in K$.

$d' > d$. This is similar to the previous case except there are no enough factors in R.H.S to accomodate the extra multiplicity of $q(X)$ and thus impossible to have such (d', d) pair.

$d' = d$. In this case, we can simplify and rearrange terms to get

$$(b_d X - a_d) p^d(X) = \sum_{i=0}^{d-1} (a_i - x b_i) p^i(X) q^{d-i}(X).$$

Since $q(X)$ divides the R.H.S and p and q are coprime, $q(X) \mid b_d X - a_d \notin K$. Thus $\deg q \leq 1$.

Thus $q(X) = aX + b$ for some $a, b \in K$. To show that $\deg p \leq 1$, we suppose NOT, and compare the degrees of two sides of equation 1. The LHS has a degree of $1 + d' \deg q + d \deg p$. The RHS has a degree of $d \deg q + d' \deg p$. This is clearly a contradiction, thus $\deg p \leq 1$.

- (11) (a) Given the extension homomorphism D in K , $D(1) = D(1/1) = 0$ and $D(1/y) = -Dy/y^2$. Then, for $x, y \in A$,

$$\begin{aligned} D(xy) &= D(x/y^{-1}) \\ &= \frac{y^{-1}Dx - xD(1/y)}{y^{-2}}. \\ &= xDy + yDx \end{aligned}$$

Next, we show that D is well-defined in K .

$$\begin{aligned} D(cx/xy) &= \frac{cyD(cx) - cxD(cy)}{c^2y^2} \\ &= \frac{cy(cDx + xDc) - cx(cDy + yDc)}{c^2y^2} \\ &= D(x/y). \end{aligned}$$

(b)

$$\begin{aligned} L(xy) &= D(xy)/xy \\ &= xDy/xy + yDx/xy \\ &= Dy/y + Dx/x \\ &= L(x) + L(y) \end{aligned}$$

(c) Applying product rule directly,

$$\begin{aligned} R'(X) &= D(c \prod_i (X - \alpha_i)^{m_i}) \\ &= c \sum_i m_i (X - \alpha_i)^{m_i-1} \prod_{j \neq i} (X - \alpha_j)^{m_j} \end{aligned}$$

Dividing this sum by $R(X)$, we get the desired sum.

- (12) (a) Let $f(X) = (a_1 X - b_1)(a_2 X - b_2) = a_1 a_2 (X - \frac{b_1}{a_1})(X - \frac{b_2}{a_2})$. The discriminant is then

$$\begin{aligned} D(f) &= (a_1 a_2)^2 \left(\frac{b_1}{a_1} - \frac{b_2}{a_2} \right)^2 \\ &= (a_2 b_1 - a_1 b_2)^2 \\ &= (a_2 b_1 + a_1 b_2)^2 - 4a_1 a_2 b_1 b_2 \\ &= b^2 - 4ac \end{aligned}$$

(b) We first prove the expression is true for $a_0 = 1$ and $f(X) = (X - t_1)(X - t_2)(X - t_3)$.

$$\begin{aligned}
s_1^2 s_2^2 &= ((t_1 + t_2 + t_3)(t_1 t_2 + t_2 t_3 + t_3 t_1))^2 \\
&= (\sum x_1^2 x_2 + 3s_3)^2 \\
&= \sum x_1^4 x_2^2 + 9s_3^2 \\
&\quad + 2(\sum x_1^3 x_2^3 + \sum x_1^4 x_2 x_3 + \sum x_1^3 x_2^2 x_3 + \sum x_1^2 x_2^2 x_3^2) \\
&\quad + 6 \sum x_1^3 x_2^2 x_3 \\
&= \sum x_1^4 x_2^2 + 2 \sum x_1^4 x_2 x_3 + 2 \sum x_1^3 x_2^3 + 8 \sum x_1^3 x_2^2 x_3 + 15 x_1^2 x_2^2 x_3^2 \\
s_1^3 s_3 &= (t_1 + t_2 + t_3)^3 s_3 \\
&= s_3 (\sum x_1^3 + 3 \sum x_1^2 x_2 + 6 \sum x_1 x_2 x_3) \\
&= \sum x_1^4 x_2 x_3 + 3 \sum x_1^3 x_2^2 x_3 + 6 \sum x_1^2 x_2^2 x_3^2 \\
s_2^3 &= (t_1 t_2 + t_2 t_3 + t_3 t_1)^3 \\
&= \sum x_1^3 x_2^3 + 3 \sum x_1^3 x_2^2 x_3 + 6 \sum x_1^2 x_2^2 x_3^2 \\
s_1 s_2 s_3 &= s_3 (t_1 + t_2 + t_3)(t_1 t_2 + t_2 t_3 + t_3 t_1) \\
&= s_3 (\sum x_1^2 x_2 + 3 x_1 x_2 x_3) \\
&= \sum x_1^3 x_2^2 x_3 + 3 x_1^2 x_2^2 x_3^2
\end{aligned}$$

where the sums are taken over all order pairs $(x_1, x_2, x_3) \in \{t_1, t_2, t_3\}^3, x_i \neq x_j$. By the definition of the discriminant, we have

$$\begin{aligned}
D_f &= (t_1 - t_2)^2 (t_2 - t_3)^2 (t_1 - t_3)^2 \\
&= \sum x_1^4 x_2^2 - 2 \sum x_1^4 x_2 x_3 - 2 \sum x_1^3 x_2^3 + 2 \sum x_1^3 x_2^2 x_3 - 6 x_1^2 x_2^2 x_3^2
\end{aligned}$$

From the above one obtains

$$D_f = s_1^2 s_2^2 - 4 s_1^3 s_3 - 4 s_2^3 + 18 s_1 s_2 s_3 - 27 s_3^2.$$

Since the above polynomial is homogenous of degree 6 and $D_{cf} = c^4 D_f$, the statement follows.

(c) $f'(X) = \sum_{i=1}^n \prod_{j \neq i} (X - t_j)$. Hence $f'(t_i) = \prod_{j \neq i} (t_i - t_j)$ where i is fixed. By definition

$$D_f = (-1)^{n(n-1)/2} \prod_{i \neq j} (t_i - t_j).$$

where the product is taken over all pairs $(i, j) i \neq j$ which is equivalent to

$$D_f = (-1)^{n(n-1)/2} \prod_{i=1}^n f'(t_i).$$

(13) (a) First suppose, f and g are coprime. By Mason-Stothers we have

$$\begin{aligned}
3 \deg f &\leq \deg f + \deg g + \deg(f^3 - g^2) - 1 \\
2 \deg g &\leq \deg f + \deg g + \deg(f^3 - g^2) - 1
\end{aligned}$$

Adding the above inequalities and simplifying, we get

$$\deg f \leq 2 \deg(f^3 - g^2) - 2$$

If f and g have common factor, then $n_0(fg) < n_0(f) + n_0(g) \leq \deg f + \deg g$. Hence the statement is proven.

- (b) The proof for case for relatively prime f, g is very similar to (a). So suppose $f = df_1, g = dg_1$ where $d \notin K$ is the greatest common divisor of f and g .

Taking $A = Ad, f = f_1, g = g_1, B = B$ in the relatively prime case, we then have the following

$$\begin{aligned}
\deg f_1 &\leq \deg Ad + \deg B + 2 \deg(Adf_1^3 + Bg_1^2) - 2 \\
&\leq \deg A + \deg d + \deg B + 2((Af^3 + Bg^2)/d^2) - 2 \\
&\leq \deg A + \deg d + \deg B + 2(\deg(Af^3 + Bg^2) - 2 \deg d) - 2 \\
&\leq \deg A + \deg B + 2 \deg(Af^3 + Bg^2) - 3 \deg d - 2 \\
&\implies \deg f \leq \deg A + \deg B + 2 \deg(Af^3 + Bg^2) - 2
\end{aligned}$$

Taking $A = d$ and $B = -1$, we get the general case for part (a).

- (c) By part (b), we may assume without loss of generality that f and g are coprime. By Mason's Theorem,

$$m \deg(f) \leq \deg(f) + \deg(g) + \deg(h) - 1$$

$$n \deg(g) \leq \deg(f) + \deg(g) + \deg(h) - 1$$

Then, with the above equations we find:

$$(n-1)(m-1) \deg(f) \leq (n-1) \deg(g) + (n-1) \deg(h) - (n-1)$$

$$(n-1) \deg(g) \leq \deg(f) + \deg(h) - 1$$

Adding these together, we find the general version:

$$((n-1)(m-1) - 1) \deg(f) \leq n \deg(h) - n$$

- (14) Let $\epsilon > 0$ be a positive number and let u, v be relatively prime non-zero integers. Let $w = u + v$. Define a polynomial f as

$$f(X) = X(X - 3u)(X + 3v)$$

Making the translation $\xi = X + v - u$, we get

$$f(\xi) = \xi^3 - \gamma_2 \xi - \gamma_3.$$

Since the discriminant is preserved under such translation, we have the following

$$D = 4\gamma_2^3 - 27\gamma_3^2 = 3^6(uvw)^2.$$

But, by the generalized Szpiro conjecture,

$$\begin{aligned}
|\gamma_2| &\ll N_o(D)^{2+\epsilon} \\
&\ll N_o((uvw)^2)^{2+\epsilon} = N_o(uvw)^{2+\epsilon},
\end{aligned}$$

and

$$|\gamma_3| \ll N_o(uvw)^{3+\epsilon}$$

If r_1, r_2, r_3 are the roots of $f(\xi)$, then

$$\begin{aligned}
\gamma_2 &= -(r_1 r_2 + r_2 r_3 + r_3 r_1) \\
&= -((v-u)(v+w) + (v+w)(-u-w) + (-u-w)(v-w)) \\
\gamma_3 &= r_1 r_2 r_3 \\
&= (v-u)(v+w)(-u-w)
\end{aligned}$$

From above, the abc conjecture follows.

(15) Define two sets:

$$A = \{p \text{ prime} : 2^{p-1} \not\equiv 1 \pmod{p^2}\}$$

$$B = \{p \text{ prime} : 2^n \equiv 1 \pmod{p} \text{ and } 2^n \not\equiv 1 \pmod{p^2}, n \geq 1\}$$

The two sets are equivalent: Let $p \in B$ and let d be the order of 2 modulo p . Since $2^d - 1 \mid 2^n - 1$, we note that $2^d \not\equiv 1 \pmod{p^2}$. At the same time, $2^{p-1} - 1 = (2^d - 1)(p-1)/d$ (since $d \mid (p-1)$), we note that $2^{p-1} - 1 \not\equiv 0 \pmod{p^2}$. Hence, $B \subseteq A$. The reverse inclusion directly follows from Fermat's little theorem. It follows that we can write any number of the form $2^n - 1$ as a product xy such that $x \in A = B$ and $y \in A^c$. If A is finite, then $x \leq \prod_{p \in A} p$. We also note that, by assumption, $N_0(y) \ll \sqrt{y}$. Assuming abc conjecture is true and taking $a = 2^n - 1$ and $b = 1$, we have

$$\begin{aligned} 2^n - 1 &= xy \\ &\ll N_0(xy)^{1+\epsilon} \\ &\ll y^{(1/2)(1+\epsilon)} \end{aligned}$$

which can only be true if y is bounded. This implies the finiteness of A^c , contradicting the infinitude of primes.

(16) Let $F(X) = a_0 + a_1X + \cdots + a_dX^d$ and $G(X) = b_0 + b_1X + \cdots + b_{d'}X^{d'}$, and assume that

$$|F| = \max_{0 \leq i \leq d} |a_i| \geq 1, \quad |G| = \max_{0 \leq j \leq d'} |b_j| \geq 1.$$

Let S be the Sylvester matrix of F and G , of size $(d + d') \times (d + d')$. The resultant R of F and G satisfies

$$R = \det(S) = \sum_{\sigma \in \mathfrak{S}_{d+d'}} \text{sgn}(\sigma) \prod_{i=1}^{d+d'} S[i, \sigma(i)].$$

Taking absolute values and using the triangle inequality,

$$|R| \leq \sum_{\sigma \in \mathfrak{S}_{d+d'}} \prod_{i=1}^{d+d'} |S[i, \sigma(i)]|.$$

Each entry of S is a coefficient of F or G , hence has absolute value at most $\max(|F|, |G|)$. More precisely, exactly d' rows contain coefficients of F and d rows contain coefficients of G , so each product contains d' occurrences of coefficients of F and d occurrences of coefficients of G . Therefore,

$$|R| \leq |F|^{d'} |G|^d (d + d')! =: B. \quad (1)$$

WLOG, we can assume $\gcd(F, G) = 1$. There exist polynomials $\phi, \psi \in \mathbb{C}[X]$ such that

$$R = \phi(X)F(X) + \psi(X)G(X),$$

with

$$\deg \phi < d', \quad \deg \psi < d.$$

Write

$$\phi(X) = \alpha_0 + \alpha_1X + \cdots + \alpha_{d'-1}X^{d'-1}, \quad \psi(X) = \beta_0 + \beta_1X + \cdots + \beta_{d-1}X^{d-1}.$$

Equating coefficients of X^k in $R = \phi F + \psi G$, and padding all coefficients outside their natural ranges with 0, we obtain the system

$$a_0\alpha_0 + b_0\beta_0 = R, \quad (2)$$

$$\sum_{i=0}^k (a_i\alpha_{k-i} + b_i\beta_{k-i}) = 0, \quad 1 \leq k \leq d + d' - 1. \quad (3)$$

From (1) and (2) we get

$$|a_0\alpha_0 + b_0\beta_0| = |R| \leq B.$$

Since $|a_0| \leq |F|$ and $|b_0| \leq |G|$, it follows that

$$|\alpha_0| + |\beta_0| \leq \frac{|R|}{\min(|a_0|, |b_0|)} \leq B. \quad (4)$$

We now prove by induction on k that

$$|\alpha_k| + |\beta_k| \leq kB \quad \text{for all } 0 \leq k \leq d + d' - 1. \quad (5)$$

The case $k = 0$ is (4). Assume the claim holds for all $0, 1, \dots, k-1$. Using (3), we have

$$a_0\alpha_k + b_0\beta_k = - \sum_{i=1}^k (a_i\alpha_{k-i} + b_i\beta_{k-i}).$$

Taking absolute values,

$$|a_0||\alpha_k| + |b_0||\beta_k| \leq \sum_{i=1}^k (|a_i||\alpha_{k-i}| + |b_i||\beta_{k-i}|).$$

Using $|a_i| \leq |F|$, $|b_i| \leq |G|$, and the induction hypothesis,

$$|a_0||\alpha_k| + |b_0||\beta_k| \leq |F| \sum_{i=1}^k |\alpha_{k-i}| + |G| \sum_{i=1}^k |\beta_{k-i}| \leq (|F| + |G|) \sum_{i=1}^k (iB).$$

Since $\sum_{i=1}^k i = \frac{k(k+1)}{2} \leq k^2$, and $|a_0|, |b_0| \geq 1$, we obtain

$$|\alpha_k| + |\beta_k| \leq kB.$$

This completes the induction and proves (5).

Now evaluate the identity $R = \phi(w)F(w) + \psi(w)G(w)$ at $X = w$:

$$|R| = |\phi(w)F(w) + \psi(w)G(w)| \leq (|\phi(w)| + |\psi(w)|)(|F(w)| + |G(w)|). \quad (6)$$

Since $|\alpha_k| + |\beta_k| \leq kB$ and $c = \max(1, |w|)$, we have

$$|\phi(w)| + |\psi(w)| \leq \sum_{k=0}^{d+d'-1} (|\alpha_k| + |\beta_k|)|w|^k \leq \sum_{k=0}^{d+d'-1} kB c^k \leq Bc^{d+d'}(d + d'). \quad (7)$$

Finally, combining (1), (6), and (7), we obtain

$$|R| \leq c^{d+d'} |F|^{d'} |G|^d (d + d')^{d+d'} (|F(w)| + |G(w)|).$$